\subsection*{\underline{Orbital Angular Momentum:}}
\begin{gather}
    \hat{L}_{x}=\hat{y} \hat{p}_{z}-\hat{z} \hat{p}_{y}, \quad \hat{L}_{y}=\hat{z} \hat{p}_{x}-\hat{x} \hat{p}_{z}, \quad \hat{L}_{z}=\hat{x} \hat{p}_{y}-\hat{y} \hat{p}_{x} \\
    {\left[\hat{L}_{x}, \hat{L}_{y}\right]=i \hbar \hat{L}_{z}, \quad\left[\hat{L}_{y}, \hat{L}_{z}\right]=i \hbar \hat{L}_{x}, \quad\left[\hat{L}_{z}, \hat{L}_{x}\right]=i \hbar \hat{L}_{y} \cdot} \\
    \hat{L}^{2} \equiv \hat{L}_{x} \hat{L}_{x}+\hat{L}_{y} \hat{L}_{y}+\hat{L}_{z} \hat{L}_{z}, \quad\left[\hat{L}^{2}, \hat{L}_{i}\right]=0 \\
    \nabla=\hat{r}\frac{\partial}{\partial r}+\hat{\theta}\frac{1}{r}\frac{\partial}{\partial \theta}+\hat{\phi}\frac{1}{r\sin\theta}\frac{\partial}{\partial \phi}\\
    \nabla^{2}=\frac{1}{r^2} \frac{\partial}{\partial r}\left( r^2\frac{\partial}{\partial r} \right)
    +\frac{1}{r^{2}\sin\theta}\frac{\partial}{\partial \theta}\left( \sin\theta\frac{\partial}{\partial\theta} \right)
    +\frac{1}{r^{2}\sin^2\theta} \left( \frac{\partial^{2}}{\partial \phi^{2}} \right)\\
    \nabla^{2}=\frac{1}{r} \frac{\partial^{2}}{\partial r^{2}} r+\frac{1}{r^{2}}\left(\frac{\partial^{2}}{\partial \theta^{2}}+\cot \theta \frac{\partial}{\partial \theta}+\frac{1}{\sin ^{2} \theta} \frac{\partial^{2}}{\partial \phi^{2}}\right) \\
    \hat{L}^{2}=-\hbar^{2}\left(\frac{\partial^{2}}{\partial \theta^{2}}+\cot \theta \frac{\partial}{\partial \theta}+\frac{1}{\sin ^{2} \theta} \frac{\partial^{2}}{\partial \phi^{2}}\right) \\
    \hat{L}_{z}=\frac{\hbar}{i} \frac{\partial}{\partial \phi} ; \quad \hat{L}_{\pm}=\hbar e^{\pm i \phi}\left(\pm \frac{\partial}{\partial \theta}+i \cot \theta \frac{\partial}{\partial \phi}\right)=\hat{L}_{x}\pm i\hat{L}_{y}
\end{gather}

\subsection*{\underline{General Momentum Operator} \fbox{$\vec{L},\, \vec{S},\, \vec{J}$}}
\begin{flalign}
     & \left[J_x, J_y\right]=i\hbar J_z
     &                                   & \left[J_z, J_x\right]=i\hbar J_y
     &                                   & \left[J_y, J_z\right]=i\hbar J_x
     &                                                                      \\
     & J^2\ket{Jm}=\hbar^2j(j+1)\ket{Jm}
     &                                   & J_z\ket{Jm}=\hbar m\ket{Jm}
     &                                   & J^2=J^2_x + J^2_y + J^2_z
\end{flalign}
\begin{gather}
    J^2 =J_\pm J_\mp + {J_z}^2\mp\hbar J_z
\end{gather}
$\ket{Jm}$ are common eigenstates of the $J^2,J_z$;\\
Thus both $J^2$ and $J_z$ are diagonal matrices for any fixed value of J, the dimension of these matrices is $(2J+1) \times (2J+1)$ since $m=-J,-J+1,\dots,J-1,J,$ (2J+1 Values).\\
$J=\frac{1}{2}\implies 2J+1=2 \implies 2\times2 \text{ matrices}.\\$
$J=1\implies 2J+1=3 \implies 3\times3\text{ matrices}.$
    \begin{flalign}    
         & J_\pm=J_x \pm iJ_y
         &                    & J_\pm\ket{J m}=\sqrt{J(J+1)-m(m\pm1)}\ket{J m\pm1}
    \end{flalign}
    so that $J_\pm$ are off diagonal matrices.\\
    We order the eigenvectors for a fixed J-value as the following:\\
$\ket{J,J}\quad\ket{J,J-1}\quad\ket{J,J-2}\quad \dots \quad\ket{J,-J}$\\
    For a fixed J here is the expectation of operator A:
    \begin{equation}
        A = 
        \left(\begin{matrix}
            \bra J A \ket J     & \bra J A \ket {J-1}   & \dots  & \bra J A \ket {-J}     \\
            \bra{ J-1} A \ket J & \bra{J-1} A \ket{J-1} & \dots  & \bra{ J-1} A \ket {-J} \\
            \vdots              & \vdots                & \vdots & \vdots                 \\
            \bra{-J} A \ket J   & \bra{-J} A \ket{J-1}  & \dots  & \bra{- J} A \ket {-J}
        \end{matrix}\right)
    \end{equation}
    in the above matrix, for a fixed J we denote $\ket{J m}=\ket m$.
    
    \subsection*{\underline{Spin Angular Momentum Operator}}
    For $j=\frac{1}{2}\implies \ket{\uparrow} = \ket{\frac{1}{2},\frac{1}{2}}; \ket{\downarrow} = \ket{\frac{1}{2},-\frac{1}{2}} then:$
\begin{flalign}
     & S_x=\frac{\hbar}{2}\left(
    \begin{matrix}
            0 & 1 \\
            1 & 0
        \end{matrix}\right) = \frac{\hbar}{2}\sigma_1
     &                                  & S_y=\frac{\hbar}{2}\left(
    \begin{matrix}
            0 & -i \\
            i & 0
        \end{matrix}\right) = \frac{\hbar}{2}\sigma_2
     &                                  & S_z=\frac{\hbar}{2}\left(
    \begin{matrix}
            1 & 0  \\
            0 & -1
        \end{matrix}\right) = \frac{\hbar}{2}\sigma_3
     &                                                                     \\
     & \left[S_x, S_y\right]=i\hbar S_z
     &                                  & \left[S_z, S_x\right]=i\hbar S_y
     &                                  & \left[S_y, S_z\right]=i\hbar S_x
     &                                                                     \\
     & S_+=S_x+iS_y
     &                                  & S_-=S_x-iS_y
     &                                                                     \\
     & S_+=\frac{\hbar}{2}\left(
    \begin{matrix}
            0 & 2 \\
            0 & 0
        \end{matrix}\right)
     &                                  & S_-=\frac{\hbar}{2}\left(
    \begin{matrix}
            0 & 0 \\
            2 & 0
        \end{matrix}\right)
\end{flalign}