\subsection*{\underline{Non-Degenerate Perturbation Theory}}

\begin{align}
     & H = H^0 + \lambda H' = H(\lambda)                                         \\
     & H(\lambda) \psi_n (\lambda) = E_n (\lambda) \psi_n (\lambda)              \\
     & \psi_n(\lambda) = \psi_n^0 + \lambda \psi_n^1 + \lambda^2 \psi_n^2+\cdots \\
     & E_n(\lambda) = E_n^0 + \lambda E_n^1 + \lambda^2 E_n^2 + \cdots           \\
     & \text{Assume }\psi_n(\lambda), \, E_n(\lambda) \text{ converges}          \\
\end{align}
\begin{align}
    \lambda^0: \quad & H^0|\psi_n^0\rangle = E_n^0 |\psi_n^0\rangle             \\
    \lambda^1: \quad & H^0|\psi_n^1\rangle + H'\psi_n^0 = E_n^0|\psi_n^1\rangle
    + E_n^1|\psi_n^0\rangle                                                     \\
    \lambda^2: \quad & H^0|\psi_n^2\rangle + H'\psi_n^1 = E_n^0|\psi_n^2\rangle
    + E_n^1|\psi_n^1\rangle + E_n^2|\psi_n^0\rangle
\end{align}

\begin{align}
    E_n^1            & = \langle\psi_n^0|H'|\psi_n^0\rangle                            \\
    |\psi_n^1\rangle & = \sum_{m\ne n} \frac{\langle \psi_m^0|H'|
    \psi_n^0\rangle}{E_n^0 - E_m^0} |\psi_m^0\rangle                                   \\
    E_n^2            & = \langle \psi_n^0 | H' | \psi_n^1\rangle                       \\
    E_n^2            & = \sum_{m\ne n} \frac{\left| \langle\psi_m^0|H'|\psi_n^0\rangle
        \right|^2}{E_n^0 - E_m^0}
\end{align}