\newpage
\subsection*{\underline{Time Dependant Perturbation:}}

\begin{gather}
	H(t) = H_o +H'(t); \hspace{0.5 cm} H_0\ket{\psi_n} = E_n\ket{\psi_n}\\
	\ket{\Psi(t)} = \sum_n{C_n(t) e^{-iE_nt/\hbar}}\ket{\psi_n}
\end{gather}
Schr√∂dinger equation

\begin{equation}
	i\hbar\frac{\partial}{\partial t}\ket{\Psi(t)} = H(t)\ket{\Psi(t)}
\end{equation}
gives:

\begin{equation}
	\left\{ \arraycolsep=1.4pt\def\arraystretch{1.5}
	\begin{array}{ll}
			\;i\hbar\dot{C_k} (t) =  \sum_n{H'_{kn}(t)e^{i\omega_{kn}t}C_n(t)}\\
			\;H'_{kn}(t) = \bra{\psi_k}\expval{H'(t)}\ket{\psi_n}\\
			\;\omega_{kn} = (E_k-E_n)/\hbar\\
	\end{array} \right.
\end{equation}
with initial condition $\ket{\psi(t_o)} = \ket{\Phi_o}$ so that:
\begin{equation}
	C_n(t_o) = \bra{\psi_n}\ket{\Phi_o}e^{-iE_nt_o/\hbar}
\end{equation}
as initial condition for the above coupled equation in $C_n(t)$

\subsection*{\underline{Two Level System:}}
\begin{gather}
	\ket{\Psi(t)} = C_a(t)e^{-iE_at/\hbar}\ket{\psi_a} + C_b(t)e^{-iE_bt/\hbar}\ket{\psi_b}\\
	H_o\ket{\psi_a} = E_a\ket{\psi_a}; \hspace{1.7 cm} H_o\ket{\psi_b} = E_b\ket{\psi_b}
\end{gather}
Gives, assuming $H_{aa} = H_{bb} = 0$,

\begin{equation}
	\left\{ \arraycolsep=1.4pt\def\arraystretch{1.5}
 	\begin{array}{ll}
			\dot{C_a} (t) =  -\frac{i}{\hbar}H'_{ab}(t)e^{-i\omega_{o}t}C_b(t)\\ 
			\dot{C_b} (t) =  -\frac{i}{\hbar}H'_{ba}(t)e^{i\omega_{o}t}C_a(t)\\
			\omega_o = \frac{E_b-E_a}{\hbar}
	\end{array} \right.
\end{equation}
Initial Condition $C_a(0) = 1; \hspace{0.5 cm} C_b(0)=0$

\subsection*{\underline{First Order Perturbation:}}
\begin{equation}
	C_b^{(1)} = -\frac{i}{\hbar}\int^t_{t_o}{H'_{ba}(t')e^{i\omega_ot'} dt'}
\end{equation}
Transition probability:
\begin{equation}
	P_{ab} = \left|C_b^{(1)}\right|^2 = \frac{1}{\hbar^2}\left|\int^t_{t_o}{H'_{ba}(t')e^{i\omega_ot'} dt'}\right|^2
\end{equation}

\section*{\underline{Sinusoidal Perturbation:}}
\begin{gather}
	\hat{H}'(\textbf{r},t) = V(\textbf{r})\cos{(\omega t)}\\
	P_{ab}(t) = |C_b(t)|^2 \approx \frac{|V_{ab}|^2}{\hbar^2}\frac{\sin^2{[(\omega_o - \omega)t/2]}}{(\omega_o-\omega)^2}\\
	\frac{dN_b}{dt} = -N_bA - N_bB_{ba}\rho(\omega_o) + N_aB_{ab}\rho(\omega_o) = 0
\end{gather}
